\textbf{Rauschbefreiungsfilter:}

\input{figures/rauschbefreiungsfilter}

\begin{align}
Z(n) &= \sum_{k=0}^{N} h_k Y(n-k)
\end{align}
\begin{align}
\min\{MSE\}  \Rightarrow 0 &\overset{!}{=} \frac{\partial MSE}{\partial h_i} = \frac{\partial \mathbb{E}[(X(n)-Z(n))^2]}{\partial h_i}\\
&= \frac{\partial \mathbb{E}[u(v(n))]}{\partial h_i} = \mathbb{E}[u'(v(n)) \cdot v'(n)] = \mathbb{E}[2 \cdot (X(n)-Z(n)) \cdot \frac{\partial v(n)}{\partial h_i}]\\
&= \mathbb{E}[2 \cdot (X(n)-Z(n)) \cdot -Y(n-i)] = -2 \cdot \mathbb{E}[(X(n)-Z(n)) \cdot Y(n-i)]\\
\Rightarrow 0 &= \mathbb{E}[X(n) \cdot Y(n-i)] - \mathbb{E}[Z(n) \cdot Y(n-i)]\\
\Leftrightarrow \mathbb{E}[X(n) \cdot Y(n-i)] &= \mathbb{E}[Z(n) \cdot Y(n-i)]\\
\Leftrightarrow R_{XY}(i) &= \mathbb{E}\left[\sum_{k=0}^{N} h_k Y(n-k) \cdot Y(n-i)\right] = \sum_{k=0}^{N} h_k \cdot \mathbb{E}[Y(n-k) \cdot Y(n-i)]\\
&= \sum_{k=0}^{N} h_k \cdot R_{YY}(i-k)\\
\text{(da, } R_{YY}(-i) = R_{YY}(i) \text{)}\\
\Rightarrow \mathbf{R_{YY}} \cdot \mathbf{h_{\text{opt}}} &= \mathbf{R_{XY}}
\end{align}

% In Matrixform
\begin{align}
\begin{bmatrix}
R_{YY}(0) & R_{YY}(1) \\
R_{YY}(1) & R_{YY}(0)
\end{bmatrix}
\begin{bmatrix}
h_{0,\text{opt}} \\
h_{1,\text{opt}}
\end{bmatrix}
&=
\begin{bmatrix}
R_{XY}(0) \\
R_{XY}(1)
\end{bmatrix}
\end{align}



\text{Filtereinstellung:}
\begin{align}
H_{opt}(\Omega) &=\frac{S_{XY}(\Omega)}{S_{YY}(\Omega)} = \frac{S_{XX}(\Omega)}{S_{XX}(\Omega) + S_{NN}(\Omega)}
\end{align}

\begin{align}
S_{XY}(\Omega) &= \mathcal{F}\{\mathbb{E}[X(n)\cdot Y(n+m)]\} = \mathcal{F}\{\mathbb{E}[X(n)\cdot(X(n+m) + N(n+m))]\}\\
R_{XN}(k) = 0 \Rightarrow \quad S_{XY}(\Omega) &= \mathcal{F}\{\mathbb{E}[X(n)\cdot X(n+m)]\} = S_{XX}(\Omega)
\end{align}
\begin{align}
S_{YY}(\Omega) &= \mathcal{F}\{\mathbb{E}[Y(n)\cdot Y(n+m)]\} = \mathcal{F}\{\mathbb{E}[(X(n) + N(n))\cdot(X(n+m) + N(n+m))]\}\\
R_{XN}(k) = 0 \Rightarrow S_{YY}(\Omega) &= \mathcal{F}\{\mathbb{E}[X(n)\cdot X(n+m)] + \mathbb{E}[N(n)\cdot N(n+m)]\} = S_{XX}(\Omega) + S_{NN}(\Omega)
\end{align}

